tests/lean/run/partial_fixpoint_induct.lean
@@ -18,6 +18,10 @@ info: loop.fixpoint_induct (motive : (Nat → Unit) → Prop) (adm : Lean.Order.
 #guard_msgs in #check loop.fixpoint_induct
 
 
+/-- error: unknown constant 'loop.partial_correctness' -/
+#guard_msgs in #check loop.partial_correctness
+
+
 def find (P : Nat → Bool) (x : Nat) : Option Nat :=
   if P x then
     some x
@@ -32,6 +36,15 @@ info: find.fixpoint_induct (P : Nat → Bool) (motive : (Nat → Option Nat) →
 -/
 #guard_msgs in #check find.fixpoint_induct
 
+/--
+info: find.partial_correctness (P : Nat → Bool) (motive : Nat → Nat → Prop)
+  (h :
+    ∀ (find : Nat → Option Nat),
+      (∀ (x r : Nat), find x = some r → motive x r) →
+        ∀ (x r : Nat), (fun x => if P x = true then some x else find (x + 1)) x = some r → motive x r)
+  (x r✝ : Nat) : find P x = some r✝ → motive x r✝
+-/
+#guard_msgs in #check find.partial_correctness
 
 def fib (n : Nat) := go 0 0 1
 where
@@ -97,3 +110,55 @@ info: dependent2''a.fixpoint_induct (m : Nat) (motive_1 : (Nat → (b : Bool) �
 
 /-- error: unknown constant 'dependent2''b.fixpoint_induct' -/
 #guard_msgs in #check dependent2''b.fixpoint_induct
+
+
+mutual
+def dependent3''a (m n : Nat) (b : Bool) : Option (if b then Nat else Bool) :=
+  if _ : b then dependent3''a m (n + 1) b else dependent3''b m m (n + m) b
+partial_fixpoint
+def dependent3''b (m k n : Nat) (b : Bool) : Option (if b then Nat else Bool) :=
+  if b then dependent3''b m k n b else dependent3''c m (.last _) (n + m) b
+partial_fixpoint
+def dependent3''c (m : Nat) (i : Fin (m+1)) (n : Nat) (b : Bool) : Option (if b then Nat else Bool) :=
+  if b then dependent3''c m i n b else dependent3''a m i b
+partial_fixpoint
+end
+
+/--
+info: dependent3''a.partial_correctness (m : Nat) (motive_1 : Nat → (b : Bool) → (if b = true then Nat else Bool) → Prop)
+  (motive_2 : Nat → Nat → (b : Bool) → (if b = true then Nat else Bool) → Prop)
+  (motive_3 : Fin (m + 1) → Nat → (b : Bool) → (if b = true then Nat else Bool) → Prop)
+  (h_1 :
+    ∀ (dependent3''a : Nat → (b : Bool) → Option (if b = true then Nat else Bool))
+      (dependent3''b : Nat → Nat → (b : Bool) → Option (if b = true then Nat else Bool)),
+      (∀ (n : Nat) (b : Bool) (r : if b = true then Nat else Bool), dependent3''a n b = some r → motive_1 n b r) →
+        (∀ (k n : Nat) (b : Bool) (r : if b = true then Nat else Bool),
+            dependent3''b k n b = some r → motive_2 k n b r) →
+          ∀ (n : Nat) (b : Bool) (r : if b = true then Nat else Bool),
+            (fun n b => if x : b = true then dependent3''a (n + 1) b else dependent3''b m (n + m) b) n b = some r →
+              motive_1 n b r)
+  (h_2 :
+    ∀ (dependent3''b : Nat → Nat → (b : Bool) → Option (if b = true then Nat else Bool))
+      (dependent3''c : Fin (m + 1) → Nat → (b : Bool) → Option (if b = true then Nat else Bool)),
+      (∀ (k n : Nat) (b : Bool) (r : if b = true then Nat else Bool), dependent3''b k n b = some r → motive_2 k n b r) →
+        (∀ (i : Fin (m + 1)) (n : Nat) (b : Bool) (r : if b = true then Nat else Bool),
+            dependent3''c i n b = some r → motive_3 i n b r) →
+          ∀ (k n : Nat) (b : Bool) (r : if b = true then Nat else Bool),
+            (fun k n b => if b = true then dependent3''b k n b else dependent3''c (Fin.last m) (n + m) b) k n b =
+                some r →
+              motive_2 k n b r)
+  (h_3 :
+    ∀ (dependent3''a : Nat → (b : Bool) → Option (if b = true then Nat else Bool))
+      (dependent3''c : Fin (m + 1) → Nat → (b : Bool) → Option (if b = true then Nat else Bool)),
+      (∀ (n : Nat) (b : Bool) (r : if b = true then Nat else Bool), dependent3''a n b = some r → motive_1 n b r) →
+        (∀ (i : Fin (m + 1)) (n : Nat) (b : Bool) (r : if b = true then Nat else Bool),
+            dependent3''c i n b = some r → motive_3 i n b r) →
+          ∀ (i : Fin (m + 1)) (n : Nat) (b : Bool) (r : if b = true then Nat else Bool),
+            (fun i n b => if b = true then dependent3''c i n b else dependent3''a (↑i) b) i n b = some r →
+              motive_3 i n b r) :
+  (∀ (n : Nat) (b : Bool) (r : if b = true then Nat else Bool), dependent3''a m n b = some r → motive_1 n b r) ∧
+    (∀ (k n : Nat) (b : Bool) (r : if b = true then Nat else Bool), dependent3''b m k n b = some r → motive_2 k n b r) ∧
+      ∀ (i : Fin (m + 1)) (n : Nat) (b : Bool) (r : if b = true then Nat else Bool),
+        dependent3''c m i n b = some r → motive_3 i n b r
+-/
+#guard_msgs in #check dependent3''a.partial_correctness
